bedrock2/src/Examples/BinarySearch.v
@@ -1,11 +1,11 @@
 Require Import bedrock2.Macros bedrock2.Syntax.
-Require Import bedrock2.StringNames bedrock2.BasicALU bedrock2.NotationsInConstr.
+Require Import bedrock2.StringNamesSyntax bedrock2.BasicALU bedrock2.NotationsInConstr.
 
 Import BinInt String.
 Local Open Scope string_scope. Local Open Scope Z_scope. Local Open Scope list_scope.
 
 Section bsearch.
-  Context {p : unique! StringNames.Syntax.parameters} {b : BasicALU.operations}.
+  Context {p : unique! StringNamesSyntax.parameters} {b : BasicALU.operations}.
   Local Coercion literal (z : Z) : expr := expr.literal z.
   Local Coercion var (x : String.string) : expr := expr.var x.
 
