bedrock2/src/Examples/Swap.v
@@ -1,11 +1,11 @@
 Require Import bedrock2.Macros bedrock2.Syntax.
-Require Import bedrock2.StringNames bedrock2.BasicALU bedrock2.NotationsInConstr.
+Require Import bedrock2.StringNamesSyntax bedrock2.BasicALU bedrock2.NotationsInConstr.
 
 Import BinInt String.
 Local Open Scope string_scope. Local Open Scope Z_scope. Local Open Scope list_scope.
 
 Section bsearch.
-  Context {p : unique! StringNames.Syntax.parameters} {b : BasicALU.operations}.
+  Context {p : unique! StringNamesSyntax.parameters} {b : BasicALU.operations}.
   Local Coercion literal (z : Z) : expr := expr.literal z.
   Local Coercion var (x : String.string) : expr := expr.var x.
 
@@ -96,7 +96,7 @@ Lemma swap_ok :
     (sep (ptsto 1 a_addr a) (sep (ptsto 1 b_addr b) R)) m ->
   WeakestPrecondition.func
     (fun _ => True) (fun _ => False) (fun _ _ => True) (fun _ _ _ _ _ => False)
-    (@swap BasicC64Syntax.parameters) t m (a_addr::b_addr::nil)
+    (@swap BasicC64Syntax.params) t m (a_addr::b_addr::nil)
     (fun t' m' rets => t=t' /\ (sep (ptsto 1 a_addr b) (sep (ptsto 1 b_addr a) R)) m' /\ rets = nil).
 Proof.
   intros. rename H into Hm.
@@ -107,8 +107,8 @@ Lemma swap_swap_ok :
   forall a_addr a b_addr b (m:map.rep (value:=@Semantics.byte _)) R t,
     (sep (ptsto 1 a_addr a) (sep (ptsto 1 b_addr b) R)) m ->
   WeakestPrecondition.func
-    (fun _ => True) (fun _ => False) (fun _ _ => True) (WeakestPrecondition.call (fun _ => True) (fun _ => False) (fun _ _ => True) [("swap", (@swap BasicC64Syntax.parameters))])
-    (@swap_swap BasicC64Syntax.parameters) t m (a_addr::b_addr::nil)
+    (fun _ => True) (fun _ => False) (fun _ _ => True) (WeakestPrecondition.call (fun _ => True) (fun _ => False) (fun _ _ => True) [("swap", (@swap BasicC64Syntax.params))])
+    (@swap_swap BasicC64Syntax.params) t m (a_addr::b_addr::nil)
     (fun t' m' rets => t=t' /\ (sep (ptsto 1 a_addr a) (sep (ptsto 1 b_addr b) R)) m' /\ rets = nil).
 Proof.
   intros. rename H into Hm.
