bedrock2/src/StringNamesSyntax.v
@@ -1,0 +1,16 @@
+Require Import bedrock2.Syntax.
+
+Require Import Coq.Strings.String.
+
+Class parameters := {
+  actname : Set;
+  bopname : Set;
+}.
+
+Instance make (p : parameters) : Syntax.parameters := {|
+  Syntax.varname := string;
+  Syntax.funname := string;
+
+  Syntax.actname := actname;
+  Syntax.bopname := bopname;
+|}.
